high/Veritas.Verifier.Merkle.fsti
@@ -81,3 +81,23 @@ val lemma_store_contains_proving_ancestor (itsl: TL.eac_log)
                                  (proving_ancestor itsl k)))
 
 
+(* if a key pk points to key k, then pk is the proving ancestor of k; (inverse of 
+ * lemma_proving_ancestor_points_to_self *)
+val lemma_points_to_implies_proving_ancestor (itsl: TL.eac_log) (k:key) (pk:key{is_proper_desc k pk}):
+  Lemma (requires (let d = desc_dir k pk in
+                   let mv = eac_merkle_value itsl pk in                   
+                   mv_points_to mv d k))
+        (ensures (proving_ancestor itsl k = pk))
+
+(* precond: k' is a proper ancestor of k, but not the proving ancestor. 
+ *          k' is also initialized (previously added)
+ * ensures: k' points to something along direction (k' -> k) and that something is an ancestor of pk
+ *) 
+val lemma_init_ancestor_ancestor_of_proving (itsl: TL.eac_log) (k:key) (k':key{is_proper_desc k k'}):
+  Lemma (requires (not (is_eac_state_init itsl k') /\
+                   k' <> proving_ancestor itsl k))
+        (ensures (let d = desc_dir k k' in
+                  let mv = eac_merkle_value itsl k' in
+                  let pk = proving_ancestor itsl k in
+                  mv_points_to_some mv d /\
+                  is_desc pk (mv_pointed_key mv d)))
